* Update AADL Actor definition, to be superseded by DEVS definition

src/aadl_dynamic_system.v
@@ -29,6 +29,226 @@
  *
  * DM21-0762
 ***)
+(* begin hide *)
+Require Import Coq.Init.Datatypes.
+Require Import Coq.ZArith.ZArith.
+Require Import Coq.Lists.List.
+Import ListNotations. (* from List *)
+
+Require Import Oqarina.core.all.
+Import NaturalTime.
+Require Import Oqarina.AADL.property_sets.all.
+Require Import Oqarina.coq_utils.all.
+Require Import Oqarina.formalisms.lts.
+Set Implicit Arguments.
+(* end hide *)
+(** %\chapter{AADL Systems} %*)
+Section Actors.
+
+    (* We revise the definition of actors as follows: intuitively, an actor is an automata-like ADT. It is defined by a state and a collection of operations that operate on this state. We define the following:
+    - [L] a set of labels that represent the different phases of the execution of the actor;
+    - [A] denote the actions that the actor may perform;
+    - [I] represents the internal state of an actor, i.e. any memory the actor needs.
+
+    An actor relies on an definition of time, inherited from [Time] formalization. *)
+
+    Variable L : Type. (* State labels *)
+    Variable A : Type. (* Actions *)
+    Variable I : Type. (* private state *)
+
+    (** An [Actor_Action] denotes an action that can be executed. We distinguish between discrete ([Dis]) and timed ([Temp]) actions. *)
+
+    Inductive Actor_Action :=
+        | Dis : A -> Actor_Action
+        | Temp : A -> Time -> Actor_Action
+        | Step : Actor_Action. (* trigger internal behavior *)
+
+    Definition Connection := list nat.
+
+    (** First, we define [Actor_State] as a placeholder to store the current state of an actor. An [Actor_State] is a tuple that holds [Current_State] which is is the curent state label (i.e. position in the underlying automata), along with a clock variable, the state of inputs and outputs variable and an internal state. [Actor_State] represents the mutable part of an actor definition. *)
+
+    Inductive Actor_State : Type := {
+        (* State information *)
+        Current_State : L;
+        Clock_Variable : Time;
+        Inputs : list Actor_Action;
+        Outputs : list Actor_Action;
+        Internal : I;
+    }.
+
+    (** Then, we define [Actor] as the immutable part of an actor definition. An [Actor] gathers the definition of initial state of an actor, and the definitions of the various operations on a state. *)
+    Inductive Actor : Type := {
+
+        (* Mutable state variable *)
+        Act_State : Actor_State;
+
+        (* Mapping functions *)
+        Prefire : Actor_State -> list Actor_State -> Actor_State;
+        Fire : Actor_State -> Actor_State;
+        Post_Fire : Actor_State -> Actor_State;
+        Deadline : L  -> Time;
+        Time_Update : L -> L;
+    }.
+
+    (** ** Operations on [Actor_State] *)
+
+    (** - [Set_Initial_Actor_State] configures the initial state of an actor. *)
+
+    Definition Set_Initial_Actor_State (Initial_State : L) (Internal : I) : Actor_State := {|
+        Current_State := Initial_State ;
+        Clock_Variable := 0;
+        Inputs := nil;
+        Outputs := nil;
+        Internal := Internal;
+    |}.
+
+    (** - [Set_State] sets the [Current_State] of an Actor *)
+
+    Definition Set_State (ast : Actor_State) (l : L) : Actor_State := {|
+        Current_State := l;
+        Clock_Variable := ast.(Clock_Variable);
+        Inputs := ast.(Inputs);
+        Outputs := ast.(Outputs);
+        Internal := ast.(Internal);
+    |}.
+
+    (** - [Peek_Input] returns one input, without dequeuing it. *)
+
+    Definition Peek_Input (ast : Actor_State) : option Actor_Action :=
+        hd_error ast.(Inputs).
+
+    (** - [Dequeue_Input] removes one input from an Actor. *)
+
+    Definition Dequeue_Input (ast : Actor_State) : Actor_State := {|
+        Current_State := ast.(Current_State);
+        Clock_Variable := ast.(Clock_Variable);
+        Inputs := tl ast.(Inputs);
+        Outputs := ast.(Outputs);
+        Internal := ast.(Internal);
+    |}.
+
+    (** - [Set_Input] adds a list of inputs to an Actor. *)
+    (* XXX should we keep a list here ... *)
+    Definition Set_Input (ast : Actor_State) (i : list Actor_Action) : Actor_State := {|
+        Current_State := ast.(Current_State);
+        Clock_Variable := ast.(Clock_Variable);
+        Inputs := Coq.Lists.List.concat [ast.(Inputs) ; i] ;
+        Outputs := ast.(Outputs);
+        Internal := ast.(Internal);
+    |}.
+
+    (** - [Set_Output] adds a list of outputs to an Actor. *)
+
+    Definition Set_Output (ast : Actor_State) (i : list Actor_Action) : Actor_State := {|
+        Current_State := ast.(Current_State);
+        Clock_Variable := ast.(Clock_Variable);
+        Inputs := ast.(Inputs);
+        Outputs := Coq.Lists.List.concat [ast.(Outputs) ; i] ;
+        Internal := ast.(Internal);
+    |}.
+
+    (** - [Peek_Output] returns one input, without dequeuing it. *)
+
+    Definition Peek_Output (ast : Actor_State) : option Actor_Action :=
+        hd_error ast.(Outputs).
+
+    (** - [Dequeue_Output] removes one input from an Actor. *)
+
+    Definition Dequeue_Output (ast : Actor_State) : Actor_State := {|
+        Current_State := ast.(Current_State);
+        Clock_Variable := ast.(Clock_Variable);
+        Inputs := ast.(Inputs);
+        Outputs := tl ast.(Outputs);
+        Internal := ast.(Internal);
+    |}.
+
+    (** - [Set_Internal] sets the internal state of an Actor *)
+
+    Definition Set_Internal (ast : Actor_State) (i : I) : Actor_State := {|
+        Current_State := ast.(Current_State);
+        Clock_Variable := ast.(Clock_Variable);
+        Inputs := ast.(Inputs);
+        Outputs := tl ast.(Outputs);
+        Internal := i;
+    |}.
+
+    (** ** Operations on [Actor] *)
+
+    Definition Set_Act_State (a : Actor) (ast : Actor_State) : Actor := {|
+        Act_State := ast;
+        Prefire := a.(Prefire);
+        Fire := a.(Fire);
+        Post_Fire := a.(Post_Fire);
+        Deadline := a.(Deadline);
+        Time_Update := a.(Time_Update);
+    |}.
+
+    Definition Actor_Set_Input (a : Actor) (i : list Actor_Action) : Actor :=
+        Set_Act_State a (Set_Input a.(Act_State) i).
+
+    Definition Actor_Dequeue_Output (a : Actor) : Actor :=
+        Set_Act_State a (Dequeue_Output a.(Act_State)).
+
+    (** An actor my perform untimed or timed action. we first define each concept separately, then we build a common action type: [Actor_Action]. Each action runs the actors functions defined in [a] on [ast] and returns an updated actor state. *)
+
+    Definition Untimed_Action (actor : Actor) (ast : Actor_State) : Actor_State :=
+        (Post_Fire actor) ((Fire actor) ast).
+
+    Definition Timed_Action (actor : Actor) (ast : Actor_State) : Actor_State :=
+        let action := Peek_Input ast in
+        match action with
+        | Some (Temp _ dt) => if dt <=? (Deadline actor) (Current_State ast) then {|
+                            Clock_Variable := (Clock_Variable ast) + dt;
+                            Current_State := (Time_Update actor) (Current_State ast);
+                            Inputs := ast.(Inputs);
+                            Outputs := ast.(Outputs);
+                            Internal := ast.(Internal);
+                        |}
+                        else
+                            ast
+        | _ => ast
+        end.
+
+    (** - [Actor_Step] executes one step, executing the action [act]. This function returns an updated [Actor_State]. XXX merge discrete actions and timed ones *)
+
+    Definition Actor_Step (a : Actor) (l : list Actor_State) : Actor :=
+        let a' := Set_Act_State a (Prefire a a.(Act_State) l) in
+        let act := Peek_Input a'.(Act_State) in
+            match act with
+                | Some (Dis _) => Set_Act_State a' (Untimed_Action a' a'.(Act_State))
+                | Some (Temp _ _) => Set_Act_State a' (Timed_Action a' a'.(Act_State))
+                | _ => a'
+            end.
+
+    (** - [Actor_Broadcast] broadcast one outpot from a to all elements of [l]. Note this function does not dequeue element from a.  *)
+
+    Definition Actor_Broadcast (a : Actor) (l : list Actor) :=
+        let act := Peek_Output a.(Act_State) in
+        match act with
+            | Some act' => map (fun x => Actor_Set_Input a [act']) l
+            | None => l
+        end.
+
+    (** - [Actor_Transfer_Output] copy one output from [src] to [dest]. Note this function does not dequeue element from [src].   *)
+
+    Definition Actor_Transfer_Output (src : Actor) (dest : Actor) :=
+        let act := Peek_Output src.(Act_State) in
+        match act with
+            | Some act' => Actor_Set_Input dest [act']
+            | None => dest
+        end.
+
+    (** - [LTS_Of] builds a labelled transition system (LTS) out of an actor. *)
+(*
+    Definition LTS_Of (a : Actor) (act : Actor_Action) (Initial_State : L) (Internal : I) : LTS_struct := {|
+        States := Actor;
+        Init := Set_Act_State a (Set_Initial_Actor_State Initial_State Internal);
+        Actions := Actor_Action;
+        Step := fun actor act => Actor_Step (Actor_Set_Input actor [act]) [] (* XXX *);
+    |}.
+*)
+End Actors.
+
 (**
 %\chapter{AADL System Category}\label{sec::aadl_system}%
 
@@ -76,90 +296,328 @@
 
 *)
 
-(* begin hide *)
-Require Import Coq.Init.Datatypes.
-Require Import Coq.ZArith.ZArith.
-Require Import Coq.Lists.List.
-Import ListNotations. (* from List *)
-
-Require Import Oqarina.formalisms.actor.
-Require Import Oqarina.core.all.
-Import NaturalTime.
-Require Import Oqarina.AADL.property_sets.all.
-Require Import Oqarina.coq_utils.utils.
-Require Import Oqarina.formalisms.lts.
-Set Implicit Arguments.
-
-Open Scope Z_scope.
-(* end hide *)
-
 (** *** Coq mechanization
 
 %\N% The following provides a Coq mechanization of the previous automata using the actor formalism. *)
 
-(** We use Coq [unit] as a system has no variable. *)
+(** [system_L] represents the labels of the state of the system hybrid automata. *)
 
-Definition system_var : Type := unit.
-
-(** %\N% The informal definition provides a direct path to the definition of states, actions and transitions.
-*)
-
-Inductive system_states : Set :=
+Inductive system_L : Set :=
     system_offline | system_starting | system_operational | system_stoping.
+Scheme Equality for system_L.
 
-Scheme Equality for system_states.
+(** [system_A] represents the set of actions that a system may perform, as per the hybrid automata defined in AADLv2.2 \S 13.3. *)
 
-Inductive system_actions : Set :=
+Inductive system_A : Set :=
     start_system | abort_system | started_system | stop_system | stopped_system.
 
-Definition system_inputs : Type := unit.
-Definition system_V : Type := unit.
-Definition system_internal : Type := unit.
-Definition system_state : Type := Actor_State system_states system_V system_internal.
+(** [system_I] is the internal state of a system, for the moment empty *)
 
-Definition system_Fire (s : system_state) (a : system_actions) : system_state := s.
+Definition system_I : Type := unit.
 
-Definition system_Post_Fire
-    (s : system_state)
-    (a : system_actions) : system_state :=
-    match s.(Current_State), a with
-        (* capture the transitions of the automata *)
-        | system_offline, start_system => (Set_State s system_starting)
-        | system_starting, started_system => (Set_State s system_operational)
-        | system_operational, stop_system => (Set_State s system_stoping)
-        | system_stoping, stopped_system => (Set_State s system_offline)
-        | system_starting, abort_system => (Set_State s system_offline)
-        | system_operational, abort_system => (Set_State s system_offline)
-        (* any other configuration is invalid *)
-        | _, _ => s
+Definition system_actions : Type := Actor_Action system_A.
+
+Definition System_Actor_Type : Type := Actor system_L system_A system_I .
+
+(** From these definition, we can build the various elements of a AADL system actor. *)
+
+Definition system_state : Type := Actor_State system_L system_A system_I.
+
+(** [System_Initial_State] is the default initial state of all system instances. *)
+
+Definition System_Initial_State : system_state :=
+    Set_Initial_Actor_State  system_A system_offline tt.
+
+Definition system_Prefire (s : system_state) (deps: list system_state) : system_state  := (* internal event queued *)
+    match s.(Current_State) with
+        | system_starting => (* XXX *)
+            match deps with
+            | [ ] => (Set_Input s [Dis started_system])
+            | _ => if andbl (map (fun x => system_L_beq system_operational (Current_State x)) deps) then (Set_Input s [Dis started_system]) else s
+            end
+        | _ => s
+    end.
+
+Definition system_executions (s : system_state) (a : system_actions) : system_state :=
+    match a with
+    | Dis a' =>
+        match s.(Current_State), a' with
+            (* capture the transitions of the automata *)
+            | system_offline, start_system => (Set_Output s [a])
+
+            (* any other configuration is invalid *)
+            | _, _ => s
+            end
+    | _ => s
+    end.
+
+Definition system_Fire (s : system_state) : system_state :=
+    let a : option system_actions := Peek_Input s in
+        match a with
+        | Some a' => system_executions s a' (* XXX *)
+        | None => s
         end.
 
-Definition system_Deadline (s : system_states) (a : system_actions) : Time :=
+Definition system_transitions (s : system_state) (a : system_actions) : system_state :=
+    match a with
+    | Dis a' =>
+        match s.(Current_State), a' with
+            (* capture the transitions of the automata *)
+            | system_offline, start_system => (Set_State s system_starting)
+            | system_starting, started_system => (Set_State s system_operational)
+            | system_operational, stop_system => (Set_State s system_stoping)
+            | system_stoping, stopped_system => (Set_State s system_offline)
+            | system_starting, abort_system => (Set_State s system_offline)
+            | system_operational, abort_system => (Set_State s system_offline)
+            (* any other configuration is invalid *)
+            | _, _ => s
+            end
+    | _ => s
+    end.
+
+Definition system_Postfire (s : system_state) : system_state :=
+    let a : option system_actions := Peek_Input s in
+    let s' := Dequeue_Input s in
+        match a with
+        | Some a' => system_transitions s' a' (* XXX *)
+        | None => s
+        end.
+
+Definition system_Deadline (s : system_L)  : Time :=
     0%nat.
 
 Definition system_Time_Update
-    (s : system_states)  (a : system_actions) (t : Time) : system_states :=
+    (s : system_L) : system_L :=
     s.
 
-Definition System_Actor : Actor system_states system_actions system_V system_internal := {|
-    Initial_State := system_offline;
+Definition System_Actor : System_Actor_Type := {|
+    Act_State := System_Initial_State;
+
+    Prefire := system_Prefire;
     Fire := system_Fire;
-    Post_Fire := system_Post_Fire;
+    Post_Fire := system_Postfire;
     Deadline := system_Deadline;
     Time_Update := system_Time_Update;
 |}.
 
-(** * Example *)
+(* Check that the initial value is correct *)
 
-(** %\N% From the previous elements, one can step a system *)
-
-Definition System_LTS := LTS_Of System_Actor tt.
-
-Definition System_LTS' := step_lts System_LTS
-    (Init System_LTS) (Dis [start_system ; started_system]).
-
-Example System_LTS'_state : Get_State System_LTS' = system_operational.
+Definition system_step0 := Actor_Step System_Actor [].
+Lemma system_step0_OK : Act_State system_step0 =
+{| Current_State := system_offline; Clock_Variable := 0%nat; Inputs := [];
+   Outputs := []; Internal := tt; |}.
 Proof.
     trivial.
 Qed.
 
+(* We inject the start_system event, the system moves to the system_starting state *)
+
+Definition system_step1 := Actor_Set_Input System_Actor [Dis start_system].
+Definition system_step1' := Actor_Step system_step1 [].
+Lemma system_step1_OK : Act_State (system_step1') =
+{| Current_State := system_starting; Clock_Variable := 0%nat; Inputs := [];
+   Outputs := [(Dis start_system)]; Internal := tt; |}.
+Proof.
+    trivial.
+Qed.
+
+(* Since there is no subcomponents, the next state is system_operational *)
+
+Definition system_step2 := Actor_Step system_step1' [].
+Lemma system_step2_OK : Act_State (system_step2) =
+{| Current_State := system_operational; Clock_Variable := 0%nat; Inputs := [];
+   Outputs := [(Dis start_system)]; Internal := tt; |}.
+Proof.
+    trivial.
+Qed.
+
+(** We now define a tree of [System_Actor] as an actor *)
+
+Section Tree.
+
+    (** We define a basic tree structure with a map-like operator *)
+
+    Inductive tree (X : Type): Type :=
+    | empty : tree X
+    | branch : identifier -> X -> list (tree X) -> tree X.
+
+    (** [map_tree] applies [f] recursively on [t] to produce a new tree. *)
+
+    Fixpoint map_tree (T : Type) (X : Type) (f : T -> X) (t : tree T) : tree X :=
+        match t with
+        | empty _ => empty X
+        | branch i a b => branch i (f a) (map (fun x => map_tree f x) b)
+        end.
+
+    Definition map_root (T : Type) (f : T -> T) (t : tree T) :=
+        match t with
+            | empty _ => empty T
+            | branch i a b => branch i (f a) b
+        end.
+
+    (** [apply_tree_id] applies [f] on node [I] *)
+
+    Fixpoint apply_tree_id (T : Type) (I : identifier) (f : T -> T) (t : tree T) :=
+        match t with
+            | empty _ => empty T
+            | branch i a b => if (identifier_beq i I) then branch i (f a) (map (fun x => apply_tree_id I f x) b) else branch i a (map (fun x => apply_tree_id I f x) b)
+        end.
+
+    (** [apply_tree] applies [f] on all nodes of [t] *)
+
+    Fixpoint apply_tree (T : Type) (f : T -> list (tree T) -> T) (t : tree T) :=
+        match t with
+            | empty _ => empty T
+            | branch i a b => branch i (f a b) (map (fun x => apply_tree f x) b)
+        end.
+
+    Fixpoint apply_tree_b (T : Type) (f : T -> list (tree T) -> bool) (t : tree T) :=
+        match t with
+            | empty _ => true
+            | branch i a b => andb (f a b) (andbl (map (fun x => apply_tree_b f x) b))
+        end.
+
+    Fixpoint apply_tree2 (T : Type) (f : T -> T -> T) (arg : option T) (t : tree T) :=
+        match t with
+            | empty _ => empty T
+            | branch i a b =>
+                match arg with
+                | None => branch i a (map (fun x => apply_tree2 f (Some a) x) b)
+                | Some a' => branch i (f a' a) (map (fun x => apply_tree2 f (Some a) x) b)
+                end
+        end.
+
+End Tree.
+
+Definition System_Actor_Tree : Type := tree System_Actor_Type.
+Definition Empty_System_Actor_Tree : System_Actor_Tree := empty System_Actor_Type.
+
+(** [Show_States] returns the actor states of the nodes of a System_Actor_Tree *)
+
+Definition Show_States (t : System_Actor_Tree) :=
+    map_tree  (fun x => Current_State (Act_State x)) t.
+
+Definition Show_States' (t : System_Actor_Tree) :=
+    map_tree  (fun x => Act_State x) t.
+
+Definition System_Actor_Tree_state : Type := Actor_State system_L system_A System_Actor_Tree.
+
+Definition System_Actor_Tree_initial_state : System_Actor_Tree_state :=
+    Set_Initial_Actor_State system_A system_offline Empty_System_Actor_Tree.
+
+Definition System_Actor_Tree_Prefire
+    (ast : System_Actor_Tree_state) (deps : list System_Actor_Tree_state):= ast.
+
+(** Executes all actors from [ast] *)
+
+Definition System_Actor_Tree_Micro_Step_exec (ast : System_Actor_Tree_state) : System_Actor_Tree_state :=
+    Set_Internal ast (map_tree (fun x => Actor_Step x []) (Internal ast)).
+
+(** Propagate outputs down the hierarchy *)
+
+Definition System_Actor_Tree_Micro_Step_comm (ast : System_Actor_Tree_state) :=
+    let ast1 := Set_Internal ast (apply_tree2 (fun x y => Actor_Transfer_Output x y)
+        None (Internal ast)) in
+        Set_Internal ast (map_tree (fun x => Actor_Dequeue_Output x) (Internal ast1)).
+
+Definition System_Actor_Tree_Fire
+    (ast : System_Actor_Tree_state) : System_Actor_Tree_state :=
+
+    (* We pass the first event from the Actor_Tree down to the root Actor for further processing. *)
+
+    let event := Peek_Input ast in (* should dequeue when all sub actors converged XXX *)
+    match event with
+    | Some evt => let tree := map_root (fun x => Actor_Set_Input x [evt]) (Internal ast) in
+                  let ast' := Set_Internal ast tree in
+                  let ast1 := System_Actor_Tree_Micro_Step_exec ast' in
+                  System_Actor_Tree_Micro_Step_comm ast1
+
+    | None => ast
+    end.
+
+Definition System_Actor_Tree_Post_Fire
+    (ast : System_Actor_Tree_state) : System_Actor_Tree_state := ast.
+
+Definition System_Actor_Tree_Deadline
+    (s : system_L)  : Time := 0%nat.
+
+Definition System_Actor_Tree_Time_Update (s : system_L) := s.
+
+Definition System_Actor_Tree_Type : Type :=
+    Actor system_L system_A System_Actor_Tree.
+
+Definition System_Actor_Tree_Actor : System_Actor_Tree_Type := {|
+    Act_State := System_Actor_Tree_initial_state ;
+
+    Prefire := System_Actor_Tree_Prefire;
+    Fire := System_Actor_Tree_Fire;
+    Post_Fire := System_Actor_Tree_Post_Fire;
+    Deadline := System_Actor_Tree_Deadline;
+    Time_Update := System_Actor_Tree_Time_Update;
+|}.
+
+Definition Instantiate_System_Actor_Tree_Actor (t : System_Actor_Tree ) :=
+    Set_Act_State System_Actor_Tree_Actor
+    (Set_Internal System_Actor_Tree_Actor.(Act_State) t).
+
+(** A toy [System_Actor_Tree]
+
+System_Actor "root"
+   |- System Actor "s1"
+        |- System_Actor "s2"
+   |- System_Actor "s3"
+
+*)
+
+Definition root_system :=
+    branch (Id "root") System_Actor
+    [ branch (Id "s1") System_Actor
+        [ branch (Id "s2") System_Actor [empty System_Actor_Type]] ;
+      branch  (Id "s3")  System_Actor [empty System_Actor_Type]].
+
+(** First. we instantiate a System_Actor_Tree  actor with [root_system], then we iterate *)
+
+Definition root_system_Actor := Instantiate_System_Actor_Tree_Actor root_system.
+
+(** [Actor_Step] performs no action, there is no input in [root_system_Actor] *)
+
+Definition root_system_step0 := Actor_Step root_system_Actor []. (* XXX *)
+Lemma step0_OK : root_system_step0 = root_system_Actor.
+Proof.
+    trivial.
+Qed.
+
+(** We inject one even in the root system, the first step will *)
+
+
+Fixpoint Iterate (T : Type) (n : nat) (f : T -> T) (x : T) :=
+    match n with
+    | 0 => x
+    | S n' => Iterate n' f (f x)
+    end.
+
+Definition root_system_step1 := Actor_Set_Input root_system_step0 [Dis start_system].
+Compute Show_States (Internal (Act_State root_system_step1)).
+
+Definition root_system_stepn := Iterate 1 (fun x => Actor_Step x []) root_system_step1.
+Compute Show_States (Internal (Act_State root_system_stepn)).
+
+
+Definition root_system_step2 := Actor_Step root_system_step1 [].
+Compute Show_States (Internal (Act_State root_system_step2)).
+
+Definition root_system_step3 := Actor_Step root_system_step2 [].
+Compute Show_States (Internal (Act_State root_system_step3)).
+
+Definition root_system_step4 := Actor_Step root_system_step3 [].
+Compute Show_States (Internal (Act_State root_system_step4)).
+
+Definition root_system_step5 := Actor_Step root_system_step4 [].
+Compute Show_States (Internal (Act_State root_system_step5)).
+
+Definition root_system_step6 := Actor_Step root_system_step5 [].
+Compute Show_States (Internal (Act_State root_system_step6)).
+
+
+Inductive AADL_Actor :=
+| Sys_Actor : System_Actor_Type -> AADL_Actor.
